wip

DesugarScopedVars.dfy
@@ -11,19 +11,21 @@ module DesugarScopedVars {
   import Util
   import opened Wrappers
 
-  predicate RelState<V>(m: map<var_name, (var_name, Ty)>, s1: map<var_name, V>, s2: map<var_name, V>)
+  predicate RelState<V>(m: map<var_name, var_name>, s1: map<var_name, V>, s2: map<var_name, V>)
   {
-    && (forall k | k in m.Keys :: 
-          && (k in s1.Keys <==> m[k].0 in s2.Keys)
-          && (k in s1.Keys ==> s1[k] == s2[m[k].0]))
+    (forall k | k in m.Keys :: Maps.Get(s1, k) == Maps.Get(s2, m[k]))
   }
 
-  predicate RelPred<A(!new)>(m: map<var_name, (var_name, Ty)>, post1: Predicate<A>, post2: Predicate<A>)
+  lemma RelStateEmpty<V>(s1: map<var_name, V> , s2: map<var_name, V>)
+  ensures RelState(map[], s1, s2)
+  { }
+
+  predicate RelPred<A(!new)>(m: map<var_name, var_name>, post1: Predicate<A>, post2: Predicate<A>)
   {
     forall s, s' | RelState(m, s, s') :: post1(s) == post2(s')
   }
 
-  predicate RelPost<A(!new)>(m: map<var_name, (var_name, Ty)>, post1: WpPostShallow<A>, post2: WpPostShallow<A>)
+  predicate RelPost<A(!new)>(m: map<var_name, var_name>, post1: WpPostShallow<A>, post2: WpPostShallow<A>)
   {
     && post1.scopes.Keys == post2.scopes.Keys
     && RelPred(m, post1.normal, post2.normal)
@@ -31,66 +33,121 @@ module DesugarScopedVars {
     && (forall lbl | lbl in post1.scopes.Keys :: RelPred(m, post1.scopes[lbl], post2.scopes[lbl]))
   }
 
-  function method MultiSubstExpr(e: Expr, varMapping: map<var_name, (var_name, Ty)>): Expr
+  function method MultiSubstExpr(e: Expr, varMapping: map<var_name, var_name>): Expr
 
-  lemma {:axiom} MultiSubstExprSpec<A(!new)>(a: absval_interp<A>, varMapping: map<var_name, (var_name, Ty)>, e: Expr, s1: state<A>, s2: state<A>)
-    requires RelState(varMapping, s1, s2)
-    requires forall x | x in e.FreeVars() :: x in varMapping.Keys || Maps.Get(s1, x) == Maps.Get(s2, x)
+  lemma MultiSubstExprSpec<A(!new)>(a: absval_interp<A>, varMapping: map<var_name, var_name>, e: Expr, s1: state<A>, s2: state<A>)
+    requires forall x | x in e.FreeVars() :: 
+      && (x in varMapping.Keys ==> Maps.Get(s1, x) == Maps.Get(s2, varMapping[x]))
+      && (x !in varMapping.Keys ==> Maps.Get(s1, x) == Maps.Get(s2, x))
     ensures EvalExpr(a, e, s1) == EvalExpr(a, MultiSubstExpr(e, varMapping), s2)
+  
+  lemma MultiSubstExprSpec2<A(!new)>(a: absval_interp<A>, varMapping: map<var_name, var_name>, e: Expr, s1: state<A>, s2: state<A>)
+    requires RelState(varMapping, s1, s2)
+    requires e.FreeVars() <= varMapping.Keys
+    ensures EvalExpr(a, e, s1) == EvalExpr(a, MultiSubstExpr(e, varMapping), s2)
+  {
+    MultiSubstExprSpec(a, varMapping, e, s1, s2);
+  }
 
-  function method SubstSimpleCmd(sc: SimpleCmd, varMapping: map<var_name, (var_name, Ty)>) : SimpleCmd
+  function method SubstSimpleCmd(sc: SimpleCmd, varMapping: map<var_name, var_name>) : SimpleCmd
   {
     match sc
     case Skip => Skip 
     case Assert(e) => Assert(MultiSubstExpr(e, varMapping))
     case Assume(e) => Assume(MultiSubstExpr(e, varMapping))
     case Assign(x, t, e) =>
-      var newLHS := if x in varMapping.Keys then varMapping[x].0 else x;
+      var newLHS := if x in varMapping.Keys then varMapping[x] else x;
       var newRHS := MultiSubstExpr(e, varMapping);
       Assign(newLHS, t, newRHS)
     case Havoc(varDecls) =>
       var varDecls' := Sequences.Map( 
-        vDecl => 
-          if vDecl.0 in varMapping.Keys then varMapping[vDecl.0] else vDecl
-
-      Havoc(varDecls)
+        (vDecl : (var_name, Ty)) => 
+          if vDecl.0 in varMapping.Keys then (varMapping[vDecl.0], vDecl.1) else vDecl,
+        varDecls);
+      Havoc(varDecls')
     case SeqSimple(c1, c2)  =>
       SeqSimple(SubstSimpleCmd(c1, varMapping), SubstSimpleCmd(c2, varMapping))
   }
 
-  lemma {:axiom} SubstSimpleCmdCorrect<A>(a: absval_interp<A>, sc: SimpleCmd, varMapping: map<var_name, (var_name, Ty)>, post: WpPostShallow<A>)
-  /*
-  ensures 
-    var sc' := SubstSimpleCmd(sc, varMapping);
-    var freshNames := map k | k in varMapping.Keys :: varMapping[k].0;
-    var updatedMap := map k | k in freshNames 
+  lemma ForallVarDeclsRel<A(!new)>(
+    a: absval_interp<A>, 
+    varDecls: seq<(var_name, Ty)>, 
+    varMapping: map<var_name, var_name>, 
+    p1: Predicate<A>,
+    p2: Predicate<A>)
+    requires RelPred(varMapping, p1, p2)
+    requires GetVarNames(varDecls) <= varMapping.Keys
+    ensures 
+      var varDecls' := Sequences.Map((vDecl : (var_name, Ty)) => (varMapping[vDecl.0], vDecl.1), varDecls);
+      RelPred(varMapping, ForallVarDeclsShallow(a, varDecls, p1), ForallVarDeclsShallow(a, varDecls, p2))
+  {
+    forall s1, s2 | RelState(varMapping, s1, s2)
+    ensures ForallVarDeclsShallow(a, varDecls, p1)(s1) == ForallVarDeclsShallow(a, varDecls, p2)(s2)
+    {
+      if |varDecls| > 0 {
 
-    forall s:state<A> :: WpShallowSimpleCmd(a, sc, post)(s) == WpShallowSimpleCmd(a, sc, post)()
-  */
+      }
+    }
+  }
+
+  lemma SubstSimpleCmdCorrect<A(!new)>(a: absval_interp<A>, sc: SimpleCmd, varMapping: map<var_name, var_name>, 
+    post1: Predicate<A>, post2: Predicate<A>)
+    requires RelPred(varMapping, post1, post2)
+    requires sc.WellFormedVars(varMapping.Keys)
+    requires Maps.Injective(varMapping)
+    ensures 
+      var sc' := SubstSimpleCmd(sc, varMapping);
+      RelPred(varMapping, WpShallowSimpleCmd(a, sc, post1), WpShallowSimpleCmd(a, sc', post2))
+  {
+    var sc' := SubstSimpleCmd(sc, varMapping);
+    var pre1 := WpShallowSimpleCmd(a, sc, post1);
+    var pre2 := WpShallowSimpleCmd(a, sc', post2);
+    forall s1:map<var_name, Val<A>>, s2 | RelState(varMapping, s1, s2)
+      ensures pre1(s1) == pre2(s2)
+    {
+      match sc
+      case Assume(e) => 
+        MultiSubstExprSpec2(a, varMapping, e, s1, s2);
+      case Assert(e) => 
+        MultiSubstExprSpec2(a, varMapping, e, s1, s2);
+      case Assign(x, t, e) =>
+        var e' := MultiSubstExpr(e, varMapping);
+        var v1Opt := EvalExpr(a, e, s1);
+        var v2Opt := EvalExpr(a, e', s2);
+        assert v1Opt == v2Opt by {
+          MultiSubstExprSpec2(a, varMapping, e, s1, s2);
+        }
+
+        if(v1Opt.Some?) {
+          var v := v1Opt.value;
+          var x' := varMapping[x];
+
+          assert RelState(varMapping, s1[x := v], s2[x' := v]) by {
+            forall k | k in varMapping.Keys 
+            ensures Maps.Get(s1[x := v], k) == Maps.Get(s2[x' := v], varMapping[k])
+            {
+              var k' := varMapping[k];
+              if k != x {
+                calc {
+                  Maps.Get(s1[x := v], k);
+                  Maps.Get(s1, k);
+                  Maps.Get(s2, k');
+                  { reveal Maps.Injective(); }
+                  Maps.Get(s2[x' := v], k');
+                }
+              }
+            }
+          }
+        }
+      case Havoc(vDecls)  => 
+
+      case _ => assume false;
+    }
+  }
 
 
   function method CreateUniqueName(names: set<var_name>): var_name
     ensures CreateUniqueName(names) !in names
-
-
-  /*
-  function method {:opaque} FoldLeft<A,T>(f: (A, T) -> A, init: A, s: seq<T>): A
-  {
-    if |s| == 0 then init
-    else FoldLeft(f, f(init, s[0]), s[1..])
-  }
-  */
-/*
-  lemma LemmaInvFoldRight<A,B>(inv: (seq<A>, B) -> bool,
-                               stp: (A, B, B) -> bool,
-                               f: (A, B) -> B,
-                               b: B,
-                               xs: seq<A>)
-    requires InvFoldRight(inv, stp)
-    requires forall a, b :: stp(a, b, f(a, b))
-    requires inv([], b)
-    ensures inv(xs, FoldRight(f, xs, b))
-*/
 
   function method CreateUniqueVarDecls(varDecls: seq<(var_name, Ty)>, usedNames: set<var_name>) : seq<(var_name,Ty)>
     ensures 
@@ -115,7 +172,7 @@ module DesugarScopedVars {
     res
   }
 
-  function method ConvertVDeclsToSubstMap(varDecls: seq<(var_name, Ty)>, varDecls': seq<(var_name, Ty)>) : map<var_name, (var_name, Ty)>
+  function method ConvertVDeclsToSubstMap(varDecls: seq<(var_name, Ty)>, varDecls': seq<(var_name, Ty)>) : map<var_name, var_name>
     requires |varDecls| == |varDecls'|
   {
     if |varDecls| == 0 then
@@ -123,7 +180,7 @@ module DesugarScopedVars {
     else
       var oldName:= varDecls[0].0;
       var newVDecl := varDecls'[0];
-      ConvertVDeclsToSubstMap(varDecls[1..], varDecls'[1..])[oldName := newVDecl]
+      ConvertVDeclsToSubstMap(varDecls[1..], varDecls'[1..])[oldName := newVDecl.0]
   }
 
   /*
@@ -132,7 +189,7 @@ module DesugarScopedVars {
   */
   function method DesugarScopedVars(
     c: Cmd, 
-    substMap: map<var_name, (var_name,Ty)>, 
+    substMap: map<var_name, var_name>, 
     usedVars: set<var_name>,
     ghost seqSubstMap: seq<(var_name, Ty)>): (Cmd, set<var_name>)
   {
@@ -157,28 +214,28 @@ module DesugarScopedVars {
     case _ => (c, usedVars) //TODO (precondition should eliminate this case)
   }
 
-  function RenameVarsState<V>(m: map<var_name, (var_name, Ty)>, s: map<var_name, V>) : map<var_name, V>
+  function RenameVarsState<V>(m: map<var_name, var_name>, s: map<var_name, V>) : map<var_name, V>
     ensures 
       var s' := RenameVarsState(m, s);
       && (forall v :: v in s.Keys && v !in m.Keys ==> s'[v] == s[v])
-      && (forall v :: v in m.Keys && m[v].0 in s.Keys ==> s'[v] == s[m[v].0])
-      && (forall v :: v in m.Keys && m[v].0 !in s.Keys ==> v !in s'.Keys)
+      && (forall v :: v in m.Keys && m[v] in s.Keys ==> s'[v] == s[m[v]])
+      && (forall v :: v in m.Keys && m[v] !in s.Keys ==> v !in s'.Keys)
   {
     var renamedState := 
-      map v | v in m.Keys && m[v].0 in s.Keys :: 
-        s[m[v].0];
+      map v | v in m.Keys && m[v] in s.Keys :: 
+        s[m[v]];
     
-    var renamedVarsWithNoTarget := set v | v in m.Keys && m[v].0 !in s.Keys;
+    var renamedVarsWithNoTarget := set v | v in m.Keys && m[v] !in s.Keys;
 
     (s - renamedVarsWithNoTarget) + renamedState
   }
 
-  function RenameVarsPred<A>(m: map<var_name, (var_name, Ty)>, p: Predicate<A>) : Predicate<A> 
+  function RenameVarsPred<A>(m: map<var_name, var_name>, p: Predicate<A>) : Predicate<A> 
   {
     s => p(RenameVarsState(m, s))
   }
 
-  function RenameVarsPost<A>(m: map<var_name, (var_name, Ty)>, post: WpPostShallow<A>) : WpPostShallow<A>
+  function RenameVarsPost<A>(m: map<var_name, var_name>, post: WpPostShallow<A>) : WpPostShallow<A>
   {
     var newScopes := map lbl | lbl in post.scopes.Keys :: RenameVarsPred(m, post.scopes[lbl]);
     WpPostShallow(RenameVarsPred(m, post.normal), RenameVarsPred(m, post.currentScope), newScopes)
@@ -187,7 +244,7 @@ module DesugarScopedVars {
   lemma DesugarScopedVarsCorrect<A(!new)>(
     a: absval_interp<A>,
     c: Cmd, 
-    substMap: map<var_name, (var_name,Ty)>, 
+    substMap: map<var_name, var_name>, 
     usedVars: set<var_name>,
     seqSubstMap: seq<(var_name, Ty)>,
     post1: WpPostShallow<A>,
